Build the Indexed_SumType format, encoders and decoders.

src/Narcissus/Formats/Derived/IndexedSumType.v
@@ -20,6 +20,7 @@ Require Import
         Fiat.Narcissus.Formats.EnumOpt
         Fiat.Narcissus.Formats.Sequence.
 Require Import
+        Fiat.Common.List.ListFacts
         Fiat.Common.ilist.
 Require Import
         Coq.Strings.String
@@ -149,7 +150,8 @@ Ltac ez_apply:=
 
 
 (*+ Fin.t *)
-(* We will use Fin.t as index *)
+(* Fin.t represent indices to an vector/array, known to be in bound.
+   We will use Fin.t as index for the sumtype and primarily use words to encode it *)
 Section Fin.
   Context {cache : Cache}.
   Context {cacheAddNat : CacheAdd cache nat}.
@@ -220,9 +222,9 @@ Section Fin.
                        else None).
   
   Lemma Fin_Decoder_Correct n sz cache_inv
-    (P_OK:  cache_inv_Property cache_inv
-    (fun P : CacheDecode -> Prop =>
-     forall (b : nat) (cd : CacheDecode), P cd -> P (addD cd b))):
+        (P_OK:  cache_inv_Property cache_inv
+                                   (fun P : CacheDecode -> Prop =>
+                                      forall (b : nat) (cd : CacheDecode), P cd -> P (addD cd b))):
     (S n < pow2 sz)%nat ->
     (CorrectDecoder AlignedByteString.ByteStringQueueMonoid
                     (Fin_invariant sz) (Fin_invariant sz) eq 
@@ -239,12 +241,107 @@ Section Fin.
     + simpl; auto.
     + extract_view.
   Qed.
+
+  (** *Aligned decoder*)
+  (* We provide two cases:
+     1. Index encoded in one Byte
+     2. Index encoded in multiple Bytes
+   *) 
+  Definition IndexedSumTypeAligneDecoderByte (n numBytes : nat):
+    AlignedDecodeM (Fin.t (S n)) numBytes:=
+    BindAlignedDecodeM
+      GetCurrentByte
+      (fun b  =>
+         (fun (b0 : word 8) =>
+            if
+              (lt_dec (@f2n (S n) (word2Fin b0)) (pow2 8) &&
+                 weqb (@fin2Word (S n) 8 (word2Fin b0)) b0)%bool
+            then (fun numBytes0 : nat => ReturnAlignedDecodeM (word2Fin b0))  numBytes
+            else ThrowAlignedDecodeM) b).
+
+  Definition IndexedSumTypeAligneDecoder_return (n sz numBytes : nat) (w: word sz):
+    AlignedDecodeM (Fin.t (S n)) numBytes:=
+    if
+      (lt_dec (@f2n (S n) (word2Fin w)) (pow2 sz) &&
+         weqb (@fin2Word (S n) sz (word2Fin w)) w)%bool
+    then (fun _ => ReturnAlignedDecodeM (word2Fin w))  numBytes
+    else ThrowAlignedDecodeM.
   
+  Definition IndexedSumTypeAligneDecoder (n szB numBytes : nat):
+    AlignedDecodeM (Fin.t (S n)) numBytes:=
+    let sz := szB * 8 in
+    BindAlignedDecodeM
+      (GetCurrentBytes szB)
+      (IndexedSumTypeAligneDecoder_return n (szB*8) numBytes).
+
+  Lemma AlignedDecodeFinByte n:
+    DecodeMEquivAlignedDecodeM
+      (Fin_Decoder n 8) (IndexedSumTypeAligneDecoderByte n).
+  Proof.
+    unfold Fin_Decoder, sequence_Decode.
+    eapply @AlignedDecodeBindCharM; intros; eauto.
+    eapply @AlignedDecode_ifb.
+    eapply @Return_DecodeMEquivAlignedDecodeM.
+  Defined.
+
+  Lemma AlignedDecodeFin (n szB: nat):
+    (forall (cd : CacheDecode) (n0 m : nat),
+        addD (addD cd n0) m = addD cd (n0 + m)) ->
+    (forall cd : CacheDecode, addD cd 0 = cd) -> 
+    DecodeMEquivAlignedDecodeM
+      (Fin_Decoder n (szB * 8)) (@IndexedSumTypeAligneDecoder n szB).
+  Proof.
+    intros; unfold Fin_Decoder, sequence_Decode,IndexedSumTypeAligneDecoder.
+    eapply Bind_DecodeMEquivAlignedDecodeM.
+    - eapply AlignedDecodeNCharM; assumption.
+    - intros.
+      eapply @AlignedDecode_ifb.
+      eapply @Return_DecodeMEquivAlignedDecodeM.
+  Defined.
+  
+  Lemma AlignedDecodeFinByte_Bind {C: Type} (n: nat):
+    forall (t: Fin.t (S n) -> DecodeM (C * ByteString) ByteString)
+      (t': Fin.t (S n) -> forall numBytes : nat, AlignedDecodeM C numBytes),
+      (forall a, DecodeMEquivAlignedDecodeM (t a) (t' a))-> 
+      DecodeMEquivAlignedDecodeM
+        (fun b cd =>
+           `(a, b0, env) <- Fin_Decoder n 8 b cd;
+         t a b0 env)
+        (fun numBytes =>
+           BindAlignedDecodeM
+             (IndexedSumTypeAligneDecoderByte n numBytes)
+             (fun a => t' a numBytes)).
+  Proof.
+    intros.
+    eapply Bind_DecodeMEquivAlignedDecodeM; eauto.
+    eapply AlignedDecodeFinByte.
+  Defined.
+  
+  Lemma AlignedDecodeFin_Bind {C: Type}:
+    (forall (cd : CacheDecode) (n0 m : nat),
+        addD (addD cd n0) m = addD cd (n0 + m)) ->
+    (forall cd : CacheDecode, addD cd 0 = cd) -> 
+    forall n szB (t: Fin.t (S n) -> DecodeM (C * ByteString) ByteString)
+      (t': Fin.t (S n) -> forall numBytes : nat, AlignedDecodeM C numBytes),
+      (forall a, DecodeMEquivAlignedDecodeM (t a) (t' a))-> 
+      DecodeMEquivAlignedDecodeM
+        (fun b cd =>
+           `(a, b0, env) <- Fin_Decoder n (szB * 8) b cd;
+         t a b0 env)
+        (fun numBytes =>
+           BindAlignedDecodeM
+             (IndexedSumTypeAligneDecoder n szB numBytes)
+             (fun a => t' a numBytes)).
+  Proof.
+    intros.
+    eapply Bind_DecodeMEquivAlignedDecodeM; eauto.
+    eapply AlignedDecodeFin; assumption.
+  Defined.
+
 End Fin.
 
 
-
-(*TThe following two tactics help in automation, solving the side
+(*The following two tactics help in automation, solving the side
 conditions of synthetizing the encoder*)
 Ltac build_evar_ilist:=
   (* NOTE: this function usees SHELVE for subgoals
@@ -282,11 +379,364 @@ Ltac split_iterate:=
   end.
 
 
-Section IndexedSumType_Modular.
 
+(*+ Vector util *)
+(* We provide aditional functionality for working with vectors.
+   Santiago: I'm surprised none of these is in the standard libraryor Fiat. Did I miss them? *)
+Section Vector.
+  Context {T: Type}.
+  Context (code_dec: forall (x y: T), {x = y} + {x <> y}). (* Decidable equality*)
+
+  Lemma Vector_In_nth:
+    forall n (v: Vector.t T n) a,
+      Vector.In a v ->
+      exists fn, Vector.nth v fn = a.
+  Proof.
+    intros.
+    dependent induction H.
+    - exists Fin.F1; reflexivity.
+    - destruct IHIn.
+      exists (Fin.FS x0).
+      rewrite <- H0. reflexivity.
+  Qed.
+
+
+  Lemma Vector_nth_In:
+    forall n fn (v: Vector.t T n),
+      Vector.In (Vector.nth v fn) v.
+  Proof.
+    intros n fn; dependent induction fn.
+    - intros; simpl.
+      dependent induction v; simpl.
+      unfold Vector.nth; simpl.
+      constructor.
+    - intros v.
+      dependent induction v; simpl.
+      clear IHv.
+      econstructor.
+      eapply IHfn.
+  Qed.
+
+  (* | Computational version of Vector.In *)
+  Fixpoint vin {n} (a: T) (v: Vector.t T n) : bool :=
+    match v with
+    | Vector.nil => false
+    | Vector.cons x aa v' => 
+        code_dec a x || vin a v'
+    end.
+  Lemma vin_Correct:
+    forall n (v:Vector.t T n)  x, (Vector.In x v <-> vin x v = true).
+  Proof.
+    split.
+    - intros HH; induction HH.
+      + simpl. destruct code_dec; auto.
+      + simpl. destruct (code_dec x x0); eauto.
+    - induction v.
+      + simpl; congruence.
+      + simpl. destruct (code_dec x h); subst.
+        * constructor.
+        * constructor 2; eauto.
+  Qed.
+
+  (* | Looks for element v in the vector and returns it's index if found *)
+  Fixpoint vindex {n} (a: T) (v: Vector.t T n): option (Fin.t n):=
+    match v as t in Vector.t _ n0 return option (Fin.t n0) with
+    | Vector.nil => None
+    | Vector.cons x aa v' =>
+        if code_dec a x then Some (Fin.F1) else
+          match vindex a v' with
+            None => None
+          | Some fn => Some (Fin.FS fn)
+          end
+    end.
+
+  (* | Finds element in list. It's only correct if the element is in the list. 
+
+     NOTICE that if the element is not in the list, it will return the index
+     (S |ls|) which is outside of the list.
+   *)
+  Fixpoint lindex_total (ls: list T) (a: T) : nat:=
+    match ls with
+      [] => 0 (* Bogus, element not found*)
+    | x::ls' => if code_dec a x then 0 else 1 + (lindex_total ls' a )
+    end.
+
+  (*  Total version of `vindex` which returns bogus values when the element is not on the list.
+     Otherwise, allways return, only correct when the value is in the list
+   *)
+  Definition vindex_total {n} (v: Vector.t T (S n)) (a: T) : Fin.t (S n):=
+    let s := lt_dec (lindex_total (Vector.to_list v) a) (S n) in
+    match s with
+    | left l => n2f l
+    | in_right => (* impossible case, index is larger than list. Give bogus result.*)
+        Fin.F1
+    end.
+  
+  (*Same as `vindex_total` but defined without lists. *)
+  Definition vindex_total' {n} (v: Vector.t T (S n)) (a: T) : Fin.t (S n).
+    induction n.
+    - inversion v; subst.
+      exact Fin.F1. (* ^ If they are not equal, returns a bogus value. *)
+    - inversion v; subst.
+      destruct (code_dec a h).
+      + subst.
+        exact Fin.F1.
+      + eapply Fin.FS.
+        eapply (IHn X).
+  Defined.
+
+
+  (* vindex_total is the inverse of Vector.nth *)
+  Lemma fint1: forall (a: Fin.t 1), a = Fin.F1.
+  Proof.
+    intros a. clear. dependent induction a; auto.
+    inversion a.
+  Qed.
+  Lemma fint1': forall (a b: Fin.t 1), a = b.
+  Proof.
+    intros. etransitivity; [| symmetry];
+              eapply fint1.
+  Qed.
+
+  (** *Prove the invertibility of Vector.nth (by  vindex_total) *)
+  (* We first need several lemmas about vectors, lists and their relation.*)
+
+  Lemma to_list_length: forall n (v: Vector.t T n),
+      (| Vector.to_list v |) = n.
+  Proof.
+    intros; induction v; auto.
+    simpl. f_equal.
+    eapply IHv.
+  Qed.
+  Lemma lindex_total_bound:
+    forall x (l: list T),
+      In x l ->
+      (lindex_total l x < (List.length l))%nat.
+  Proof.
+    intros x ls.
+    induction ls.
+    - intros ?; exfalso; assumption.
+    - simpl; intros.
+      destruct (code_dec x a).
+      + subst. lia.
+      + simpl.
+        destruct H.
+        * exfalso; auto.
+        * eapply IHls in H. lia.
+  Qed.
+
+  Lemma f2n_FS: forall n (a: Fin.t n),
+      S (f2n a) = f2n (Fin.FS a).
+  Proof.
+    intros.
+    remember (let (i, P) := Fin.to_nat a in
+              exist (fun i0 : nat => (i0 < S n)%nat) (S i) (lt_n_S i n P)) as XX.
+    unfold f2n.
+    match goal with
+    | |- ?lhs = proj1_sig ?rhs =>
+        replace rhs with XX; subst XX
+    end.
+    remember (Fin.to_nat a) as A.
+    destruct A; reflexivity.
+    reflexivity.
+  Qed.
+  Lemma vector_to_list_nth:
+    forall n (v: Vector.t T n) a (def:T),
+      Vector.nth v a = List.nth (f2n a) (Vector.to_list v) def.
+  Proof.
+    intros n. induction n.
+    - intros. inversion a.
+    - intros.
+      dependent induction v; subst; try solve[intros; inversion a].
+      clear IHv.
+      dependent induction a; try clear IHa.
+      + reflexivity.
+      + replace (Vector.nth (Vector.cons T h n v) (Fin.FS a)) with
+          (Vector.nth v a) by reflexivity.
+        erewrite (IHn v a).
+        replace (f2n (Fin.FS a)) with (S (f2n a)).
+        reflexivity.
+
+        clear.
+        eapply f2n_FS.
+  Qed.
+
+  Lemma lindex_total_nth:
+    forall ls m def, NoDup ls ->
+                (m < (| ls |))%nat ->  
+                lindex_total ls (nth m ls def) = m.
+  Proof.
+    clear.
+    induction ls. 
+    - simpl. intros; lia.
+    - intros.
+      destruct m; simpl.
+      + destruct (code_dec a a); auto. exfalso; auto. 
+      + assert (NoDup (a::ls)) by auto. 
+        assert (HH:( m < (| ls |))%nat) by (simpl in *; lia).
+        destruct (code_dec (nth m ls def) a); cycle 1.
+        * simpl in *. rewrite IHls; auto.
+          inversion H1; assumption.
+        * inversion H1; subst.
+          contradict H4.
+          eapply nth_In. auto.
+  Qed.
+
+  Definition Vector_NoDup {n} (v: Vector.t T (S n)):=
+    NoDup (Vector.to_list v).
+
+  Instance CInv_Vectornth {n:nat} (codes: Vector.t T (S n)):
+    ConditionallyInvertible (Vector.nth codes) (constant (Vector_NoDup codes)) (vindex_total codes).
+  Proof. constructor.
+         unfold vindex_total.
+         pose proof (to_list_length _ codes); intros.
+         remember (Vector.to_list codes) as ls.
+         remember (Vector.nth codes a) as x.
+         match goal with
+         | |- (match ?x with left _ => _ | _ => _ end) = _ => destruct x 
+         end.
+         - eapply f2n_inj; rewrite f2n_n2f.
+           erewrite (vector_to_list_nth _ _ _ x) in Heqx.
+           rewrite Heqx.
+           remember (f2n a) as m.
+           rewrite <- Heqls.
+           eapply lindex_total_nth.
+           { subst ls. eauto. }
+           subst.
+           rewrite H.
+           eapply f2n_ok.
+
+         - (* simple case, where the index has to be the last element.
+            NO! this case should be impossible, the index is at least the length of the list.
+            *)
+           unshelve erewrite vector_to_list_nth in Heqx; try eassumption.
+           contradiction n0.
+           rewrite <- H.
+           eapply (lindex_total_bound x ls).
+           rewrite Heqx, <- Heqls. eapply nth_In.
+           rewrite H.
+           apply f2n_ok.
+  Qed.
+  (* also invertible in the other sense*)
+  Lemma CInv_vindex_total {n:nat} (codes: Vector.t T (S n)) (HNoDup: Vector_NoDup codes):
+    ConditionallyInvertible (vindex_total codes) (fun x => Vector.In x codes) (Vector.nth codes) .
+  Proof.
+    econstructor; intros.
+    eapply Vector_In_nth in H as [? H].
+    rewrite <- H.
+    edestruct @CInv_Vectornth.
+    rewrite CInvRoundTrip; auto.
+  Qed.
+
+End Vector.
+
+
+(*+ Vector index *)
+(* Another way to encode Fin.t, is to use a vector of "codes". The
+index is determined by the position of the code on the vector.
+
+ We implement a generic version (abstracting the
+ type/format/encoder/decoder of the "code") and then instantiate it
+ with Words. A future implementation, for XML, would include tags in String.
+ *)
+Section VectorIndex.
+  Context {cache : Cache}.
+  Context {cacheAddNat : CacheAdd cache nat}.
+
+  (*Codes are a decidable type*)
+  Context {codeT: Type}. (* The type of the code *)
+  Context (code_dec: forall (x y: codeT), {x = y} + {x <> y}). (* Decidable equality*)
+  
+  (* Format, Encoder, Decoder *)
+  Context {codeFormat : FormatM codeT  ByteString}.
+  Context (codeEncoder : forall sz : nat, @AlignedEncodeM cache codeT sz).
+  Context (codeInv: codeT -> Prop)
+          (codeDecode: DecodeM (codeT * ByteString) ByteString).
+
+  (** *The Format*)
+  Definition Format_VectorIndex {n} (codes: Vector.t codeT n) : FormatM (Fin.t n) ByteString:=
+    codeFormat ◦ Vector.nth codes.
+
+  
+  (** *The encoder*)
+  Definition VectroIndex_AlignEncoder {n} (codes: Vector.t codeT n):= Projection_AlignedEncodeM codeEncoder (Vector.nth codes).
+
+  Lemma VectorIndex_Encoder_Correct:
+    forall {n} (codes: Vector.t codeT n),
+      CorrectAlignedEncoder codeFormat codeEncoder -> 
+      CorrectAlignedEncoder (Format_VectorIndex codes) (VectroIndex_AlignEncoder codes).
+  Proof.
+    unfold Format_VectorIndex.
+    intros; eapply CorrectAlignedEncoderProjection;
+      eassumption.
+  Qed.
+  Let blah {T}: T -> Prop := constant True.
+  (** *The Decoder*)
+  Existing Instance CInv_Vectornth.
+  Lemma VectorIndex_Decoder_Correct:
+    forall {n} (codes: Vector.t codeT (S n)) cache_inv
+      BOGUS,
+      Vector_NoDup codes ->
+      (cache_inv_Property cache_inv (constant True) ->
+       CorrectDecoder ByteStringQueueMonoid codeInv 
+                      codeInv eq codeFormat codeDecode cache_inv codeFormat) ->
+      let invariant := fun x => codeInv (Vector.nth codes x) in 
+      { decoder & prod (CorrectDecoder AlignedByteString.ByteStringQueueMonoid
+                                       invariant invariant eq 
+                                       (Format_VectorIndex codes)
+                                       decoder cache_inv (Format_VectorIndex codes))
+                       (BOGUS decoder)}.
+  Proof.
+    intros * HNoDup HCorrectDec.
+    do 2 econstructor.
+    - unfold Format_VectorIndex.
+      normalize_format. 
+      eapply format_sequence_correct.
+      + do 2 instantiate(1:=constant True). 
+        unfold cache_inv_Property. auto.
+      + eassumption.
+      + intros; apply H. 
+      + unshelve instantiate(1:=_).
+        intros code.
+        intros ??. 
+        exact (if vin code_dec code codes then Some (vindex_total code_dec codes code, H, X) else None).
+        simpl; intros. eapply CorrectDecoderEmpty.
+        * (* build_fully_determined_type *)
+          unfold Heading.Domain, Tuple.GetAttribute, Tuple.GetAttributeRaw,
+            Basics.compose in *; simpl in *.
+          let a' := fresh in
+          intros a'; try destruct a'; destruct_conjs.
+          unfold Heading.Domain, Tuple.GetAttribute, Tuple.GetAttributeRaw in *;
+            simpl in *; intros. decompose_source_predicate. subst_projections.
+          subst_invertible. try rewrite H3. reflexivity.
+        * unfold IsProj.
+          unfold General.decides.
+          destruct (vin code_dec v1 codes) eqn:HH.
+          -- eapply vin_Correct in HH.
+             simpl.
+             match goal with
+               |- context [codeInv ?x] =>
+                 assert (HH0:x = v1);
+                 [| rewrite HH0]
+             end; try split; eauto.
+             apply CInv_vindex_total; auto.
+          -- intros [_ Hfalse].
+  Abort. (* We can achieve the same goal with Enum, already proved.
+            For now this is not needed. 
+          *)
+  
+End VectorIndex.
+
+
+
+(*+ Modular Indexed SumTypes *)
+  (* | The IndexedSumType is modular over any other format/encoder/decoder for Fin.t *)
+  
   (* This lemma is dumplicated from AlignedAutomation.v to avoid circular references.
      TODO: Refactor to reduce duplicagtion. 
    *)
+Section IndexedSumType_Modular.
+
   Lemma encoder_empty_cache_OK {S1 S2}
         (format_A : FormatM S1 ByteString)
         (format_B : FormatM S2 ByteString)
@@ -333,34 +783,34 @@ Section IndexedSumType_Modular.
   Definition IndexedSumType_AlignEncoder:= False.
 
   Definition encoder_IndexedSumType {n} 
-                 (encode_fin: forall sz0 : nat,
-                     @AlignedEncodeM EmptyStore.test_cache (Fin.t n) sz0)
-      {types}
-                 (encoders: ilist (B:= fun T : Type =>
-                                         forall sz : nat, @AlignedEncodeM _ T sz) types)
-                 (sz : nat)
-        : @AlignedEncodeM _ (@SumType n types) sz
-        :=
-     (Projection_AlignedEncodeM encode_fin
-                                (SumType_index types) sz>>
-                                AlignedEncodeSumType encoders sz)%AlignedEncodeM.
+             (encode_fin: forall sz0 : nat,
+                 @AlignedEncodeM EmptyStore.test_cache (Fin.t n) sz0)
+             {types}
+             (encoders: ilist (B:= fun T : Type =>
+                                     forall sz : nat, @AlignedEncodeM _ T sz) types)
+             (sz : nat)
+    : @AlignedEncodeM _ (@SumType n types) sz
+    :=
+    (Projection_AlignedEncodeM encode_fin
+                               (SumType_index types) sz>>
+                               AlignedEncodeSumType encoders sz)%AlignedEncodeM.
   
   Lemma IndexedSumType_Encoder_Correct:
     forall (n sz:nat)
-      types
-      formats
-      (encoders: ilist (B:= fun T : Type =>
-                              forall sz : nat, @AlignedEncodeM _ T sz) types)
-      (Encoders_OK:   IterateBoundedIndex.Iterate_Dep_Type_BoundedIndex
-                        (fun idx : Fin.t n =>
-                           CorrectAlignedEncoder (ith (B:=fun T : Type =>
-                                                            FormatM T ByteString)
-                                                      formats idx)
-                                                 (ith encoders idx)))
-      format_fin
-      (encode_fin: forall sz0 : nat,
-          @AlignedEncodeM EmptyStore.test_cache (Fin.t n) sz0)
-      (EncodeFin_OK: CorrectAlignedEncoder format_fin encode_fin), 
+           types
+           formats
+           (encoders: ilist (B:= fun T : Type =>
+                                   forall sz : nat, @AlignedEncodeM _ T sz) types)
+           (Encoders_OK:   IterateBoundedIndex.Iterate_Dep_Type_BoundedIndex
+                             (fun idx : Fin.t n =>
+                                CorrectAlignedEncoder (ith (B:=fun T : Type =>
+                                                                 FormatM T ByteString)
+                                                           formats idx)
+                                                      (ith encoders idx)))
+           format_fin
+           (encode_fin: forall sz0 : nat,
+               @AlignedEncodeM EmptyStore.test_cache (Fin.t n) sz0)
+           (EncodeFin_OK: CorrectAlignedEncoder format_fin encode_fin), 
       CorrectAlignedEncoder (@format_IndexedSumType n sz types formats format_fin)
                             (encoder_IndexedSumType encode_fin encoders).
   Proof.
@@ -383,11 +833,11 @@ Section IndexedSumType_Modular.
   
   (** *The Decoder*)
   Definition decoder_IndexedSumType 
-      {n types}
-      (decoder_fin: DecodeM (Fin.t n * ByteString) ByteString)
-      (decoders: ilist (B:= fun T => DecodeM (T * ByteString) ByteString) types)
-      := sequence_Decode decoder_fin
-                        (decode_SumType types decoders).
+             {n types}
+             (decoder_fin: DecodeM (Fin.t n * ByteString) ByteString)
+             (decoders: ilist (B:= fun T => DecodeM (T * ByteString) ByteString) types)
+    := sequence_Decode decoder_fin
+                       (decode_SumType types decoders).
 
   Lemma IndexedSumType_Decoder_Correct (n sz: nat)
         types
@@ -400,8 +850,8 @@ Section IndexedSumType_Modular.
         (cache_invariants: Vector.t (Ensembles.Ensemble (CacheDecode -> Prop)) n)
         (cache_invariants_OK: cache_inv_Property cache_inv (fun P =>
                                                               P_inv1 P /\
-                              IterateBoundedIndex.Iterate_Ensemble_BoundedIndex
-                                (fun idx : Fin.t n => Vector.nth cache_invariants idx P)))
+                                                                IterateBoundedIndex.Iterate_Ensemble_BoundedIndex
+                                                                  (fun idx : Fin.t n => Vector.nth cache_invariants idx P)))
         (decoders: ilist (B:= fun T => DecodeM (T * ByteString) ByteString) types)
         (decoders_OK: IterateBoundedIndex.Iterate_Ensemble_BoundedIndex
                         (fun idx : Fin.t n =>
@@ -419,13 +869,13 @@ Section IndexedSumType_Modular.
     let source_pred st :=
       view_fin (SumType_index types st) /\ ith invariants (SumType_index types st) (SumType_proj types st) in
     CorrectDecoder ByteStringQueueMonoid
-                    source_pred source_pred
-                    eq 
-                    (@format_IndexedSumType n sz types formats format_fin)
-                    (decoder_IndexedSumType decoder_fin decoders)
-                    cache_inv
-                    (@format_IndexedSumType n sz types formats format_fin)
-                    .
+                   source_pred source_pred
+                   eq 
+                   (@format_IndexedSumType n sz types formats format_fin)
+                   (decoder_IndexedSumType decoder_fin decoders)
+                   cache_inv
+                   (@format_IndexedSumType n sz types formats format_fin)
+  .
   Proof.
     unfold format_IndexedSumType.
     eapply format_sequence_correct; cycle 1.
@@ -468,16 +918,20 @@ Section IndexedSumType_Modular.
       clear - cache_invariants_OK.
       eapply cache_invariants_OK.
   Qed.
-   
-     
+  
+  
 End IndexedSumType_Modular.
 
-Section IndexedSumType.
 
+
+(*+ Indexed SumTypes with Words *)
+(* Specialized to using words directly to encode the Fin.t index. *)
+Section IndexedSumTypeWord.
+  (* In this section, we specialize the fromat/encoder/decoder to use a word as index. *)
 
   (** *The Format*)
   (*We will abstract the format for Fin.t to make proofs modular and simpler. *)
-  Definition format_IndexedSumType_full {m} (sz: nat)
+  Definition format_IndexedSumType_word {m} (sz: nat)
              {types : Vector.t Type m}
              (formats : ilist (B := fun T => FormatM T ByteString) types)
     : FormatM (SumType types) ByteString
@@ -487,21 +941,21 @@ Section IndexedSumType.
   
   Lemma IndexedSumType_Encoder_Correct':
     forall (n sz:nat)
-      types
-      formats
-      (* The following two hyp are inherited from encoding words*)
-      (addE_addE_plus : forall (ce : CacheFormat) (n m : nat),
-                    addE (addE ce n) m = addE ce (n + m))
-      (addE_0 : forall ce : CacheFormat, addE ce 0 = ce)
-      (encoders: ilist (B:= fun T : Type =>
-                              forall sz : nat, @AlignedEncodeM _ T sz) types)
-      (Encoders_OK:   IterateBoundedIndex.Iterate_Dep_Type_BoundedIndex
-                        (fun idx : Fin.t n =>
-                           CorrectAlignedEncoder (ith (B:=fun T : Type =>
-                                                             FormatM T ByteString)
-                                                        formats idx)
-                                                  (ith encoders idx))), 
-      CorrectAlignedEncoder (format_IndexedSumType_full (sz * 8) formats)
+           types
+           formats
+           (* The following two hyp are inherited from encoding words*)
+           (addE_addE_plus : forall (ce : CacheFormat) (n m : nat),
+               addE (addE ce n) m = addE ce (n + m))
+           (addE_0 : forall ce : CacheFormat, addE ce 0 = ce)
+           (encoders: ilist (B:= fun T : Type =>
+                                   forall sz : nat, @AlignedEncodeM _ T sz) types)
+           (Encoders_OK:   IterateBoundedIndex.Iterate_Dep_Type_BoundedIndex
+                             (fun idx : Fin.t n =>
+                                CorrectAlignedEncoder (ith (B:=fun T : Type =>
+                                                                 FormatM T ByteString)
+                                                           formats idx)
+                                                      (ith encoders idx))), 
+      CorrectAlignedEncoder (format_IndexedSumType_word (sz * 8) formats)
                             (encoder_IndexedSumType (Fin_AlignEncoder sz) encoders).
   Proof.
     intros.
@@ -515,45 +969,45 @@ Section IndexedSumType.
       (decoders: ilist (B:= fun T => DecodeM (T * ByteString) ByteString) types)
       := @decoder_IndexedSumType (S n) types (Fin_Decoder n sz) decoders.
 
-  Lemma IndexedSumType_Decoder_Correct' (n sz: nat):
+  Lemma IndexedSumTypeWord_Decoder_Correct (n sz: nat):
     let m:= S n in
     forall types
-      formats
-      cache_inv
-      (* inherited from fin_format*)
-      (Bound_OK: (S n < pow2 sz)%nat) 
-      (* inherited from formta words*)
-      (invariants: ilist (B:= fun T => T -> Prop) types)
-      (cache_invariants: Vector.t (Ensembles.Ensemble (CacheDecode -> Prop)) m) 
-      (cache_invariants_OK:
-        cache_inv_Property cache_inv
-                           (fun P : CacheDecode -> Prop =>
-                              (fun P0 : CacheDecode -> Prop =>
-                                 forall (b : nat) (cd : CacheDecode), P0 cd -> P0 (addD cd b)) P /\
-                                IterateBoundedIndex.Iterate_Ensemble_BoundedIndex
-                                  (fun idx : Fin.t (S n) => Vector.nth cache_invariants idx P)))
-      (decoders: ilist (B:= fun T => DecodeM (T * ByteString) ByteString) types)
-      (decoders_OK: IterateBoundedIndex.Iterate_Ensemble_BoundedIndex
-                      (fun idx : Fin.t m =>
-                         cache_inv_Property cache_inv (Vector.nth cache_invariants idx) ->
-                         CorrectDecoder BinLib.ByteStringQueueMonoid 
-                                        (ith invariants idx) (ith invariants idx) eq 
-                                        (ith formats idx) (ith decoders idx) cache_inv 
-                                        (ith formats idx)))
+           formats
+           cache_inv
+           (* inherited from fin_format*)
+           (Bound_OK: (S n < pow2 sz)%nat) 
+           (* inherited from formta words*)
+           (invariants: ilist (B:= fun T => T -> Prop) types)
+           (cache_invariants: Vector.t (Ensembles.Ensemble (CacheDecode -> Prop)) m) 
+           (cache_invariants_OK:
+             cache_inv_Property cache_inv
+                                (fun P : CacheDecode -> Prop =>
+                                   (fun P0 : CacheDecode -> Prop =>
+                                      forall (b : nat) (cd : CacheDecode), P0 cd -> P0 (addD cd b)) P /\
+                                     IterateBoundedIndex.Iterate_Ensemble_BoundedIndex
+                                       (fun idx : Fin.t (S n) => Vector.nth cache_invariants idx P)))
+           (decoders: ilist (B:= fun T => DecodeM (T * ByteString) ByteString) types)
+           (decoders_OK: IterateBoundedIndex.Iterate_Ensemble_BoundedIndex
+                           (fun idx : Fin.t m =>
+                              cache_inv_Property cache_inv (Vector.nth cache_invariants idx) ->
+                              CorrectDecoder BinLib.ByteStringQueueMonoid 
+                                             (ith invariants idx) (ith invariants idx) eq 
+                                             (ith formats idx) (ith decoders idx) cache_inv 
+                                             (ith formats idx)))
     ,
       let source_pred st :=
         (f2n (SumType_index types st) < pow2 sz)%nat /\ ith invariants (SumType_index types st) (SumType_proj types st) in
       CorrectDecoder ByteStringQueueMonoid
                      source_pred source_pred
                      eq 
-                     (format_IndexedSumType_full sz formats)
+                     (format_IndexedSumType_word sz formats)
                      (@decoder_IndexedSumType_full n sz types decoders)
                      cache_inv
-                     (format_IndexedSumType_full sz formats)
+                     (format_IndexedSumType_word sz formats)
   .
   Proof.
     intros.
-    unfold format_IndexedSumType_full, decoder_IndexedSumType_full.
+    unfold format_IndexedSumType_word, decoder_IndexedSumType_full.
     subst m.
     eapply (IndexedSumType_Decoder_Correct (S n) sz types formats cache_inv  (Format_Fin sz) (fun st:Fin.t (S n) => (f2n st  < pow2 sz)%nat)); eauto.
 
@@ -561,36 +1015,149 @@ Section IndexedSumType.
     
   Qed.
 
-End IndexedSumType.
-
-
-
-
-(*Ltacs to apply the lemma*)
-
-
-(* Use `subst_pow2; lia` instead *)
-(* (* Solves equations with small powers of two `pow2`. *)
-(*    For powers larger than 8 we'll neet a simpler way to evaluate `pow2` *) *)
-(* Ltac pow2_lia:= *)
-(*   try rewrite pow2_1; *)
-(*   try rewrite pow2_2; *)
-(*   try rewrite pow2_3; *)
-(*   try rewrite pow2_4; *)
-(*   try rewrite pow2_5; *)
-(*   try rewrite pow2_6; *)
-(*   try rewrite pow2_7; *)
-(*   try rewrite pow2_8; lia. *)
-
+  (* An easy way to build ilists invariants with all  `constant True` *)
+  Fixpoint ilist_constant_T {n: nat} (types: Vector.t Type n):
+    ilist  (B:= fun T => T -> Prop) types:=
+    match types as t0 in (Vector.t _ n0) return @ilist _  _ n0 t0 with
+      Vector.nil => tt
+    | @Vector.cons _ a n0 types0 =>
+        {| prim_fst := constant True; prim_snd := (@ilist_constant_T n0 types0) |}
+    end.
+  
+End IndexedSumTypeWord.
 
 
 (* Creates all the veriables inside ilists and vectors to apply the lemma*)
-Ltac apply_IndexedSumType_Decoder_Correct' n types :=
+Ltac apply_IndexedSumType_Decoder_Correct n types :=
+        let types' := eval unfold types in types in
+          ilist_of_evar (fun T => DecodeM (T * ByteString) ByteString) types'
+                        ltac:(fun decoders' =>
+                                ilist_of_evar (fun T : Type => T -> Prop) types'
+                                              ltac:(fun invariants' =>
+                                                      Vector_of_evar n (Ensembles.Ensemble (CacheDecode -> Prop))
+                                                                     ltac:(fun cache_invariants' =>
+                                                                             eapply IndexedSumType_Decoder_Correct with
+                                                                             (cache_invariants := cache_invariants')
+                                                                             (invariants := invariants')
+                                                                             (decoders := decoders')))).
+
+Ltac apply_IndexedSumTypeWord_Decoder_Correct n types :=
   let types' := eval unfold types in types in 
     ilist_of_evar (fun T => DecodeM (T * ByteString) ByteString) types'
                   ltac:(fun decoders' =>
                           Vector_of_evar n (Ensembles.Ensemble (CacheDecode -> Prop))
                                          ltac:(fun cache_invariants'  =>
-                                                 eapply IndexedSumType_Decoder_Correct' with
+                                                 eapply IndexedSumTypeWord_Decoder_Correct with
                                                  (cache_invariants:= cache_invariants')
                                                  (decoders:= decoders'))).
+
+      
+
+Global Opaque format_IndexedSumType.
+
+
+
+
+(*+ Indexed SumTypes with Enums *)
+(* Specialized to using words directly to encode the Fin.t index. *)
+Section IndexedSumTypeEnum.
+  (* In this section, we specialize the fromat/encoder/decoder to use a Enums as index. *)
+
+  Context {sz: nat}. (* Size of words *)
+  Context (n:nat) (codes: Vector.t (word sz) (S n)).
+  
+  (** *The Format*)
+  (*We will abstract the format for Fin.t to make proofs modular and simpler. *)
+  Definition format_IndexedSumType_enum
+             {types : Vector.t Type (S n)}
+             (formats : ilist (B := fun T => FormatM T ByteString) types)
+    : FormatM (SumType types) ByteString
+    := format_IndexedSumType sz types formats (@format_enum n _ _ _ _ _ sz codes).
+  
+(*   (** *The encoder*) *)
+(*   Lemma IndexedSumType_enum_Encoder_Correct': *)
+(*     forall (n sz:nat) *)
+(*            types *)
+(*            formats *)
+(*            (* The following two hyp are inherited from encoding words*) *)
+(*            (addE_addE_plus : forall (ce : CacheFormat) (n m : nat), *)
+(*                addE (addE ce n) m = addE ce (n + m)) *)
+(*            (addE_0 : forall ce : CacheFormat, addE ce 0 = ce) *)
+(*            (encoders: ilist (B:= fun T : Type => *)
+(*                                    forall sz : nat, @AlignedEncodeM _ T sz) types) *)
+(*            (Encoders_OK:   IterateBoundedIndex.Iterate_Dep_Type_BoundedIndex *)
+(*                              (fun idx : Fin.t n => *)
+(*                                 CorrectAlignedEncoder (ith (B:=fun T : Type => *)
+(*                                                                  FormatM T ByteString) *)
+(*                                                            formats idx) *)
+(*                                                       (ith encoders idx))),  *)
+(*       CorrectAlignedEncoder (format_IndexedSumType_word (sz * 8) formats) *)
+(*                             (encoder_IndexedSumType (Fin_AlignEncoder sz) encoders). *)
+(*   Proof. *)
+(*     intros. *)
+(*     apply IndexedSumType_Encoder_Correct; auto. *)
+(*     apply Fin_Encoder_Correct; auto. *)
+(*   Qed. *)
+  
+(*   (** *The Decoder*) *)
+(*   Let decoder_IndexedSumType_full  *)
+(*       {n} sz {types} *)
+(*       (decoders: ilist (B:= fun T => DecodeM (T * ByteString) ByteString) types) *)
+(*       := @decoder_IndexedSumType (S n) types (Fin_Decoder n sz) decoders. *)
+
+(*   Lemma IndexedSumTypeWord_Decoder_Correct (n sz: nat): *)
+(*     let m:= S n in *)
+(*     forall types *)
+(*            formats *)
+(*            cache_inv *)
+(*            (* inherited from fin_format*) *)
+(*            (Bound_OK: (S n < pow2 sz)%nat)  *)
+(*            (* inherited from formta words*) *)
+(*            (invariants: ilist (B:= fun T => T -> Prop) types) *)
+(*            (cache_invariants: Vector.t (Ensembles.Ensemble (CacheDecode -> Prop)) m)  *)
+(*            (cache_invariants_OK: *)
+(*              cache_inv_Property cache_inv *)
+(*                                 (fun P : CacheDecode -> Prop => *)
+(*                                    (fun P0 : CacheDecode -> Prop => *)
+(*                                       forall (b : nat) (cd : CacheDecode), P0 cd -> P0 (addD cd b)) P /\ *)
+(*                                      IterateBoundedIndex.Iterate_Ensemble_BoundedIndex *)
+(*                                        (fun idx : Fin.t (S n) => Vector.nth cache_invariants idx P))) *)
+(*            (decoders: ilist (B:= fun T => DecodeM (T * ByteString) ByteString) types) *)
+(*            (decoders_OK: IterateBoundedIndex.Iterate_Ensemble_BoundedIndex *)
+(*                            (fun idx : Fin.t m => *)
+(*                               cache_inv_Property cache_inv (Vector.nth cache_invariants idx) -> *)
+(*                               CorrectDecoder BinLib.ByteStringQueueMonoid  *)
+(*                                              (ith invariants idx) (ith invariants idx) eq  *)
+(*                                              (ith formats idx) (ith decoders idx) cache_inv  *)
+(*                                              (ith formats idx))) *)
+(*     , *)
+(*       let source_pred st := *)
+(*         (f2n (SumType_index types st) < pow2 sz)%nat /\ ith invariants (SumType_index types st) (SumType_proj types st) in *)
+(*       CorrectDecoder ByteStringQueueMonoid *)
+(*                      source_pred source_pred *)
+(*                      eq  *)
+(*                      (format_IndexedSumType_word sz formats) *)
+(*                      (@decoder_IndexedSumType_full n sz types decoders) *)
+(*                      cache_inv *)
+(*                      (format_IndexedSumType_word sz formats) *)
+(*   . *)
+(*   Proof. *)
+(*     intros. *)
+(*     unfold format_IndexedSumType_word, decoder_IndexedSumType_full. *)
+(*     subst m. *)
+(*     eapply (IndexedSumType_Decoder_Correct (S n) sz types formats cache_inv  (Format_Fin sz) (fun st:Fin.t (S n) => (f2n st  < pow2 sz)%nat)); eauto. *)
+
+(*     intros; eapply Fin_Decoder_Correct; eauto. *)
+    
+(*   Qed. *)
+
+(*   (* An easy way to build ilists invariants with all  `constant True` *) *)
+(*   Fixpoint ilist_constant_T {n: nat} (types: Vector.t Type n): *)
+(*     ilist  (B:= fun T => T -> Prop) types:= *)
+(*     match types as t0 in (Vector.t _ n0) return @ilist _  _ n0 t0 with *)
+(*       Vector.nil => tt *)
+(*     | @Vector.cons _ a n0 types0 => *)
+(*         {| prim_fst := constant True; prim_snd := (@ilist_constant_T n0 types0) |} *)
+(*     end. *)
+  
+End IndexedSumTypeEnum.
